renaming CyclicPerm to CircularShift

CircularShift_R.v
@@ -15,25 +15,25 @@ Require Import misc.
 
 (** Definition *)
 
-Definition cond_cyclicPerm l := {' (n, m) : _ & l = cfun (S n) (S m) } + { l = Id (length l) }.
+Definition cond_circularShift l := {' (n, m) : _ & l = cfun (S n) (S m) } + { l = Id (length l) }.
 
-Lemma Id_cond_cyclic : forall n, cond_cyclicPerm (Id n).
+Lemma Id_cond_circular : forall n, cond_circularShift (Id n).
 Proof. intros; right; now rewrite seq_length. Qed.
 
-Lemma cfun_S_cond_cyclic : forall n m, cond_cyclicPerm (cfun (S n) (S m)).
+Lemma cfun_S_cond_circular : forall n m, cond_circularShift (cfun (S n) (S m)).
 Proof. intros; left; now split with (n, m). Qed.
 
-Lemma cfun_cond_cyclic : forall n m, cond_cyclicPerm (cfun n m).
+Lemma cfun_cond_circular : forall n m, cond_circularShift (cfun n m).
 Proof.
 intros n m; destruct n ; [ | destruct m ].
 - unfold cfun; simpl; rewrite app_nil_r.
-  apply Id_cond_cyclic.
+  apply Id_cond_circular.
 - unfold cfun; simpl; rewrite seq_cons.
-  apply Id_cond_cyclic.
-- apply cfun_S_cond_cyclic.
+  apply Id_cond_circular.
+- apply cfun_S_cond_circular.
 Qed.
 
-Lemma cond_cyclic_cfun_lt {l} : cond_cyclicPerm l -> {' (n, m) : _ & l = cfun n m & m = 0 -> n = 0}.
+Lemma cond_circular_cfun_lt {l} : cond_circularShift l -> {' (n, m) : _ & l = cfun n m & m = 0 -> n = 0}.
 Proof.
 intros [[[n m] Heqcp] | Heqcp]; subst.
 - now exists (S n, S m).
@@ -42,16 +42,16 @@ intros [[[n m] Heqcp] | Heqcp]; subst.
   + now intros _.
 Qed.
 
-Lemma cond_cyclic_cfun {l} : cond_cyclicPerm l -> {' (n, m) : _ & l = cfun n m }.
-Proof. intros Hc; destruct (cond_cyclic_cfun_lt Hc) as [(n,m) Heq Hlt]; now exists (n,m). Qed.
+Lemma cond_circular_cfun {l} : cond_circularShift l -> {' (n, m) : _ & l = cfun n m }.
+Proof. intros Hc; destruct (cond_circular_cfun_lt Hc) as [(n,m) Heq Hlt]; now exists (n,m). Qed.
 
-Lemma cond_cyclic_is_perm {l} : cond_cyclicPerm l -> is_perm l = true.
-Proof. intros Hc; destruct (cond_cyclic_cfun Hc) as [(n, m) Heq]; subst; apply cfun_is_perm. Qed.
+Lemma cond_circular_is_perm {l} : cond_circularShift l -> is_perm l = true.
+Proof. intros Hc; destruct (cond_circular_cfun Hc) as [(n, m) Heq]; subst; apply cfun_is_perm. Qed.
 
-Definition CyclicPerm_R {A} (l1 l2 : list A) :=
-  { f : _ & cond_cyclicPerm f & prod (length f = length l1) (l2 = f ∘ l1) }.
+Definition CircularShift_R {A} (l1 l2 : list A) :=
+  { f : _ & cond_circularShift f & prod (length f = length l1) (l2 = f ∘ l1) }.
 
-Infix "~°~" := CyclicPerm_R (at level 70).
+Infix "~°~" := CircularShift_R (at level 70).
 
 
 Section Properties.
@@ -59,20 +59,20 @@ Section Properties.
 Context {A : Type}.
 Implicit Types la lb lc : list A.
 
-Lemma CyclicPerm_R_commu : forall la lb, la ++ lb ~°~ lb ++ la.
+Lemma CircularShift_R_commu : forall la lb, la ++ lb ~°~ lb ++ la.
 Proof.
 intros l1 l2.
 split with (cfun (length l1) (length l2)); [ | split ].
-- apply cfun_cond_cyclic.
+- apply cfun_cond_circular.
 - length_lia.
 - symmetry; apply app_cfun_eq.
 Defined.
 
-Lemma decomp_CyclicPerm_R : forall la lb,
+Lemma decomp_CircularShift_R : forall la lb,
   la ~°~ lb -> {' (la', lb') : _ & la' ++ lb' = la & lb' ++ la' = lb }.
 Proof.
 intros l1 l2 [f Hc [Hlen Heq]]; subst.
-destruct (cond_cyclic_cfun Hc) as [(n,m) Heq]; subst.
+destruct (cond_circular_cfun Hc) as [(n,m) Heq]; subst.
 exists (Id n ∘ l1, seq n m ∘ l1).
 - rewrite <- app_nat_fun_app, <- seq_app.
   rewrite cfun_length in Hlen; rewrite Hlen.
@@ -80,24 +80,24 @@ exists (Id n ∘ l1, seq n m ∘ l1).
 - symmetry; apply app_nat_fun_app.
 Qed.
 
-Instance CyclicPerm_Perm_R : Proper (CyclicPerm_R ==> (@Perm_R A)) (fun a => a).
-Proof. intros l1 l2 [f Hc [Hlen Heq]]; subst; now exists f; [ apply cond_cyclic_is_perm | ]. Defined.
+Instance CircularShift_Perm_R : Proper (CircularShift_R ==> (@Perm_R A)) (fun a => a).
+Proof. intros l1 l2 [f Hc [Hlen Heq]]; subst; now exists f; [ apply cond_circular_is_perm | ]. Defined.
 
-Instance CyclicPerm_R_refl : Reflexive (@CyclicPerm_R A).
+Instance CircularShift_R_refl : Reflexive (@CircularShift_R A).
 Proof.
   intros l.
   split with (Id (length l)); repeat split.
-  - apply Id_cond_cyclic.
+  - apply Id_cond_circular.
   - length_lia.
   - symmetry; apply app_Id.
 Defined.
 
-Instance CyclicPerm_R_sym : Symmetric (@CyclicPerm_R A).
+Instance CircularShift_R_sym : Symmetric (@CircularShift_R A).
 Proof.
 intros l l' [f Hc [Hlen Heq]]; subst.
-destruct (cond_cyclic_cfun Hc) as [(n,m) Heq]; subst.
+destruct (cond_circular_cfun Hc) as [(n,m) Heq]; subst.
 exists (cfun m n); [ | split ].
-- apply cfun_cond_cyclic.
+- apply cfun_cond_circular.
 - rewrite app_nat_fun_length by assumption.
   length_lia.
 - rewrite <- asso_app_nat_fun, cfun_inv.
@@ -105,53 +105,53 @@ exists (cfun m n); [ | split ].
   symmetry; apply app_Id.
 Defined.
 
-Instance CyclicPerm_R_trans : Transitive (@CyclicPerm_R A).
+Instance CircularShift_R_trans : Transitive (@CircularShift_R A).
 Proof.
 intros l1 l2 l3 [c1 HC1 [Hlen1 Heq1]] [c2 HC2 [Hlen2 Heq2]]; subst.
-destruct (cond_cyclic_cfun HC1) as [(i,j) Heq]; subst.
-destruct (cond_cyclic_cfun HC2) as [(k,l) Heq]; subst.
+destruct (cond_circular_cfun HC1) as [(i,j) Heq]; subst.
+destruct (cond_circular_cfun HC2) as [(k,l) Heq]; subst.
 rewrite app_nat_fun_length in Hlen2 by assumption.
 rewrite_all cfun_length.
 destruct (cfun_cfun i j k l) as [(n,m) Heq]; [ lia | ].
 rewrite <- asso_app_nat_fun, Heq.
 exists (cfun n m); [ | split ].
-- apply cfun_cond_cyclic.
+- apply cfun_cond_circular.
 - rewrite <- Heq.
   rewrite app_nat_fun_length; rewrite ? cfun_length; lia.
 - reflexivity.
 Defined.
 
-Global Instance CyclicPerm_R_equiv : Equivalence (@CyclicPerm_R A).
+Global Instance CircularShift_R_equiv : Equivalence (@CircularShift_R A).
 Proof.
 split.
-- apply CyclicPerm_R_refl.
-- apply CyclicPerm_R_sym.
-- apply CyclicPerm_R_trans.
+- apply CircularShift_R_refl.
+- apply CircularShift_R_sym.
+- apply CircularShift_R_trans.
 Qed.
 
-Lemma CyclicPerm_R_app : forall la lb lc, la ++ lb ~°~ lc -> lb ++ la ~°~ lc.
-Proof. intros l1 l2 l3 HC; now transitivity (l1 ++ l2); [ apply CyclicPerm_R_commu | ]. Defined.
+Lemma CircularShift_R_app : forall la lb lc, la ++ lb ~°~ lc -> lb ++ la ~°~ lc.
+Proof. intros l1 l2 l3 HC; now transitivity (l1 ++ l2); [ apply CircularShift_R_commu | ]. Defined.
 
-Lemma CyclicPerm_R_app_rot : forall la lb lc, la ++ lb ++ lc ~°~ lb ++ lc ++ la.
-Proof. intros l1 l2 l3; rewrite (app_assoc l2); apply CyclicPerm_R_commu. Defined.
+Lemma CircularShift_R_app_rot : forall la lb lc, la ++ lb ++ lc ~°~ lb ++ lc ++ la.
+Proof. intros l1 l2 l3; rewrite (app_assoc l2); apply CircularShift_R_commu. Defined.
 
-Lemma CyclicPerm_R_last : forall a la, a :: la ~°~ la ++ a :: nil.
-Proof. intros a la; change (a :: la) with ((a :: nil) ++ la); apply CyclicPerm_R_commu. Defined.
+Lemma CircularShift_R_last : forall a la, a :: la ~°~ la ++ a :: nil.
+Proof. intros a la; change (a :: la) with ((a :: nil) ++ la); apply CircularShift_R_commu. Defined.
 
-Lemma CyclicPerm_R_swap : forall a b : A, a :: b :: nil ~°~ b :: a :: nil.
-Proof. intros a b; change (b :: a :: nil) with ((b :: nil) ++ (a :: nil)); apply CyclicPerm_R_last. Defined.
+Lemma CircularShift_R_swap : forall a b : A, a :: b :: nil ~°~ b :: a :: nil.
+Proof. intros a b; change (b :: a :: nil) with ((b :: nil) ++ (a :: nil)); apply CircularShift_R_last. Defined.
 
-Lemma CyclicPerm_R_cons : forall la a lb, la ++ a :: nil ~°~ lb -> a :: la ~°~ lb.
-Proof. intros l1 a l2 HC; now apply (CyclicPerm_R_app l1 (a :: nil)). Defined.
+Lemma CircularShift_R_cons : forall la a lb, la ++ a :: nil ~°~ lb -> a :: la ~°~ lb.
+Proof. intros l1 a l2 HC; now apply (CircularShift_R_app l1 (a :: nil)). Defined.
 
-Lemma CyclicPerm_R_morph_cons : forall P : list A -> Prop,
-  (forall a l, P (l ++ a :: nil) -> P (a :: l)) ->  Proper (CyclicPerm_R ==> Basics.impl) P.
+Lemma CircularShift_R_morph_cons : forall P : list A -> Prop,
+  (forall a l, P (l ++ a :: nil) -> P (a :: l)) ->  Proper (CircularShift_R ==> Basics.impl) P.
 Proof.
 enough (forall P : list A -> Prop,
-         (forall a l, P (l ++ a :: nil) -> P (a :: l)) -> forall l1 l2, CyclicPerm_R l1 l2 -> P l1 -> P l2)
+         (forall a l, P (l ++ a :: nil) -> P (a :: l)) -> forall l1 l2, CircularShift_R l1 l2 -> P l1 -> P l2)
   as Himp by now intros P HP l1 l2 HC H; apply Himp with l1.
 intros P HP l1 l2 HC.
-apply decomp_CyclicPerm_R in HC as [[l0 l3] Heql1 Heql2]; subst.
+apply decomp_CircularShift_R in HC as [[l0 l3] Heql1 Heql2]; subst.
 revert l0 ; induction l3 using rev_ind ; intros l0 HPl.
 - now rewrite app_nil_r in HPl.
 - rewrite app_assoc in HPl.
@@ -160,48 +160,48 @@ revert l0 ; induction l3 using rev_ind ; intros l0 HPl.
   now apply IHl3.
 Qed.
 
-Lemma CyclicPerm_R_nil : forall la, nil ~°~ la -> la = nil.
-Proof. intros; now apply Perm_R_nil, CyclicPerm_Perm_R. Qed.
+Lemma CircularShift_R_nil : forall la, nil ~°~ la -> la = nil.
+Proof. intros; now apply Perm_R_nil, CircularShift_Perm_R. Qed.
 
-Lemma CyclicPerm_R_nil_cons : forall la a, nil ~°~ a :: la -> False.
-Proof. intros l a HC; apply CyclicPerm_R_nil in HC; inversion HC. Qed.
+Lemma CircularShift_R_nil_cons : forall la a, nil ~°~ a :: la -> False.
+Proof. intros l a HC; apply CircularShift_R_nil in HC; inversion HC. Qed.
 
-Lemma CyclicPerm_R_one : forall a b : A, a :: nil ~°~ b :: nil -> a = b.
-Proof. intros; now apply Perm_R_length_1, CyclicPerm_Perm_R. Qed.
+Lemma CircularShift_R_one : forall a b : A, a :: nil ~°~ b :: nil -> a = b.
+Proof. intros; now apply Perm_R_length_1, CircularShift_Perm_R. Qed.
 
-Lemma CyclicPerm_R_two : forall a1 a2 b1 b2 : A,
+Lemma CircularShift_R_two : forall a1 a2 b1 b2 : A,
   a1 :: a2 :: nil ~°~ b1 :: b2 :: nil -> { a1 = b1 /\ a2 = b2 } +  { a1 = b2 /\ a2 = b1 }.
-Proof. intros; now apply Perm_R_length_2, CyclicPerm_Perm_R. Qed.
+Proof. intros; now apply Perm_R_length_2, CircularShift_Perm_R. Qed.
 
-Lemma CyclicPerm_R_one_inv : forall la a, a :: nil ~°~ la -> la = a :: nil.
-Proof. intros; now apply Perm_R_length_1_inv, CyclicPerm_Perm_R. Qed.
+Lemma CircularShift_R_one_inv : forall la a, a :: nil ~°~ la -> la = a :: nil.
+Proof. intros; now apply Perm_R_length_1_inv, CircularShift_Perm_R. Qed.
 
-Lemma CyclicPerm_R_two_inv : forall a b la,
+Lemma CircularShift_R_two_inv : forall a b la,
   a :: b :: nil ~°~ la -> { la = a :: b :: nil } + { la = b :: a :: nil }.
-Proof. intros; now apply Perm_R_length_2_inv, CyclicPerm_Perm_R. Qed.
+Proof. intros; now apply Perm_R_length_2_inv, CircularShift_Perm_R. Qed.
 
-Lemma CyclicPerm_R_vs_elt_inv : forall a la lb lc,
+Lemma CircularShift_R_vs_elt_inv : forall a la lb lc,
   la ~°~ lb ++ a :: lc -> {'(l1', l2') | lc ++ lb = l2' ++ l1' & la = l1' ++ a :: l2' }.
 Proof.
   intros a l l1 l2 HC.
-  apply decomp_CyclicPerm_R in HC as [[l0 l3] H1 H2]; subst.
+  apply decomp_CircularShift_R in HC as [[l0 l3] H1 H2]; subst.
   symmetry in H2.
   dichot_Type_elt_app_exec H2 ; subst.
   - exists (l0 ++ l1, l) ; simpl ; now rewrite <- app_assoc.
   - exists (l4, l2 ++ l3) ; simpl ; now rewrite <- app_assoc.
 Qed.
 
-Lemma CyclicPerm_R_vs_cons_inv : forall a la lb,
+Lemma CircularShift_R_vs_cons_inv : forall a la lb,
   la ~°~ a :: lb -> {'(l1', l2') | lb = l2' ++ l1' & la = l1' ++ a :: l2' }.
 Proof.
   intros a l l1 HC.
   rewrite <- (app_nil_l (a::_)) in HC.
-  apply CyclicPerm_R_vs_elt_inv in HC; destruct HC as [(l' & l'') H1 H2].
+  apply CircularShift_R_vs_elt_inv in HC; destruct HC as [(l' & l'') H1 H2].
   rewrite app_nil_r in H1 ; subst.
   now exists (l', l'').
 Qed.
 
-Lemma CyclicPerm_R_app_app_inv : forall la lb lc ld,
+Lemma CircularShift_R_app_app_inv : forall la lb lc ld,
   la ++ lb ~°~ lc ++ ld ->
      {'(l1',l2',l3',l4') : _ & prod (la ~°~ l1' ++ l3') (lb ~°~ l2' ++ l4')
                              & prod (lc ~°~ l1' ++ l2') (ld ~°~ l3' ++ l4') }
@@ -215,127 +215,127 @@ Lemma CyclicPerm_R_app_app_inv : forall la lb lc ld,
                      & l1' ~°~ l2' }.
 Proof.
 intros l1 l2 l3 l4 HC.
-apply decomp_CyclicPerm_R in HC as [[lx ly] Hx Hy].
+apply decomp_CircularShift_R in HC as [[lx ly] Hx Hy].
 dichot_Type_app_exec Hx ; dichot_Type_app_exec Hy ; subst.
 - left ; left ; left ; right.
   exists (l ++ l0 , l0 ++ l).
-  + split; rewrite <- ? app_assoc; apply CyclicPerm_R_app_rot.
-  + apply CyclicPerm_R_commu.
+  + split; rewrite <- ? app_assoc; apply CircularShift_R_app_rot.
+  + apply CircularShift_R_commu.
 - dichot_Type_app_exec Hy0 ; subst.
   + left ; left ; left ; left.
-    exists (l, l0, lx, l5); split; try apply CyclicPerm_R_commu; reflexivity.
+    exists (l, l0, lx, l5); split; try apply CircularShift_R_commu; reflexivity.
   + left ; right.
     exists (l1 ++ lx , lx ++ l1).
-    * split; rewrite <- ? app_assoc; apply CyclicPerm_R_app_rot.
-    * apply CyclicPerm_R_commu.
+    * split; rewrite <- ? app_assoc; apply CircularShift_R_app_rot.
+    * apply CircularShift_R_commu.
 - dichot_Type_app_exec Hy1 ; subst.
   + left ; left ; right.
     exists (ly ++ l2, l2 ++ ly).
-    * split; rewrite <- ? app_assoc; apply CyclicPerm_R_app_rot.
-    * apply CyclicPerm_R_commu.
+    * split; rewrite <- ? app_assoc; apply CircularShift_R_app_rot.
+    * apply CircularShift_R_commu.
   + left ; left ; left ; left.
-    exists (l, ly, l3, l0); split; try apply CyclicPerm_R_commu; reflexivity.
+    exists (l, ly, l3, l0); split; try apply CircularShift_R_commu; reflexivity.
 - right.
   exists (l5 ++ l0, l0 ++ l5).
-  + split; rewrite <- ? app_assoc; apply CyclicPerm_R_app_rot.
-  + apply CyclicPerm_R_commu.
+  + split; rewrite <- ? app_assoc; apply CircularShift_R_app_rot.
+  + apply CircularShift_R_commu.
 Defined.
 
 (** [rev], [in], [map], [Forall], [Exists], etc. *)
-Instance CyclicPerm_R_rev : Proper (CyclicPerm_R ==> CyclicPerm_R) (@rev A).
+Instance CircularShift_R_rev : Proper (CircularShift_R ==> CircularShift_R) (@rev A).
 Proof.
 intro l ; induction l ; intros l' HC.
-- apply CyclicPerm_R_nil in HC ; subst ; apply CyclicPerm_R_refl.
-- apply CyclicPerm_R_sym in HC.
-  apply CyclicPerm_R_vs_cons_inv in HC.
+- apply CircularShift_R_nil in HC ; subst ; apply CircularShift_R_refl.
+- apply CircularShift_R_sym in HC.
+  apply CircularShift_R_vs_cons_inv in HC.
   destruct HC as [(l1 & l2) Heq1 Heq2] ; subst.
   simpl ; rewrite ? rev_app_distr ; simpl.
   rewrite <- app_assoc.
-  apply CyclicPerm_R_commu.
+  apply CircularShift_R_commu.
 Defined.
 
-Instance CyclicPerm_R_in (a : A) : Proper (CyclicPerm_R ==> Basics.impl) (In a).
+Instance CircularShift_R_in (a : A) : Proper (CircularShift_R ==> Basics.impl) (In a).
 Proof with try eassumption.
 intros l l' HC Hin.
 eapply Perm_R_in...
-apply CyclicPerm_Perm_R...
+apply CircularShift_Perm_R...
 Qed.
 
 End Properties.
 
 
-Instance CyclicPerm_R_map {A B} (f : A -> B) : Proper (CyclicPerm_R ==> CyclicPerm_R) (map f).
+Instance CircularShift_R_map {A B} (f : A -> B) : Proper (CircularShift_R ==> CircularShift_R) (map f).
 Proof.
 intros l l' HC.
-apply decomp_CyclicPerm_R in HC as [[lx ly] Hx Hy]; subst ; rewrite ? map_app.
-apply CyclicPerm_R_commu.
+apply decomp_CircularShift_R in HC as [[lx ly] Hx Hy]; subst ; rewrite ? map_app.
+apply CircularShift_R_commu.
 Defined.
 
-Lemma CyclicPerm_R_map_inv {A B} : forall(f : A -> B) l1 l2,
+Lemma CircularShift_R_map_inv {A B} : forall(f : A -> B) l1 l2,
   l1 ~°~ map f l2 -> { l : _ & l1 = map f l & l2 ~°~ l }.
 Proof with try assumption.
 induction l1 ; intros l2 HP.
 - exists nil ; try reflexivity.
   simpl ; destruct l2...
-  + apply CyclicPerm_R_refl.
-  + apply CyclicPerm_R_nil in HP.
+  + apply CircularShift_R_refl.
+  + apply CircularShift_R_nil in HP.
     inversion HP.
-- apply CyclicPerm_R_sym in HP.
+- apply CircularShift_R_sym in HP.
   assert (Heq := HP).
-  apply CyclicPerm_R_vs_cons_inv in Heq.
+  apply CircularShift_R_vs_cons_inv in Heq.
   destruct Heq as [(l3 & l4) Heq1 Heq2].
   simpl in Heq1 ; simpl in Heq2 ; symmetry in Heq2.
   decomp_map_Type Heq2 ; subst ; simpl.
   exists (x :: l6 ++ l0).
   + simpl ; rewrite ? map_app ; reflexivity.
-  + apply (CyclicPerm_R_commu l0).
+  + apply (CircularShift_R_commu l0).
 Defined.
 
-Lemma CyclicPerm_R_image {A B} : forall (f : A -> B) a l l',
+Lemma CircularShift_R_image {A B} : forall (f : A -> B) a l l',
   a :: l ~°~ map f l' -> { a' | a = f a' }.
 Proof.
 intros f a l l' HP.
 eapply Perm_R_image.
-apply CyclicPerm_Perm_R ; eassumption.
+apply CircularShift_Perm_R ; eassumption.
 Qed.
 
-Instance CyclicPerm_R_Forall {A} (P : A -> Prop) :
-  Proper (CyclicPerm_R ==> Basics.impl) (Forall P).
+Instance CircularShift_R_Forall {A} (P : A -> Prop) :
+  Proper (CircularShift_R ==> Basics.impl) (Forall P).
 Proof with try eassumption.
 intros l1 l2 HC HF.
 eapply Perm_R_Forall...
-apply CyclicPerm_Perm_R...
+apply CircularShift_Perm_R...
 Qed.
 
-Instance CyclicPerm_R_Exists {A} (P : A -> Prop) :
-  Proper (CyclicPerm_R ==> Basics.impl) (Exists P).
+Instance CircularShift_R_Exists {A} (P : A -> Prop) :
+  Proper (CircularShift_R ==> Basics.impl) (Exists P).
 Proof with try eassumption.
 intros l1 l2 HC HE.
 eapply Perm_R_Exists...
-apply CyclicPerm_Perm_R...
+apply CircularShift_Perm_R...
 Qed.
 
-Instance CyclicPerm_R_Forall_Type {A} (P : A -> Type) :
-  Proper (CyclicPerm_R ==> Basics.arrow) (Forall_Type P).
+Instance CircularShift_R_Forall_Type {A} (P : A -> Type) :
+  Proper (CircularShift_R ==> Basics.arrow) (Forall_Type P).
 Proof with try eassumption.
 intros l1 l2 HC HF.
 eapply Perm_R_Forall_Type...
-apply CyclicPerm_Perm_R...
+apply CircularShift_Perm_R...
 Qed.
 
-Instance CyclicPerm_R_Exists_Type {A} (P : A -> Type) :
-  Proper (CyclicPerm_R ==> Basics.arrow) (Exists_Type P).
+Instance CircularShift_R_Exists_Type {A} (P : A -> Type) :
+  Proper (CircularShift_R ==> Basics.arrow) (Exists_Type P).
 Proof with try eassumption.
 intros l1 l2 HC HE.
 eapply Perm_R_Exists_Type...
-apply CyclicPerm_Perm_R...
+apply CircularShift_Perm_R...
 Qed.
 
-Lemma CyclicPerm_R_Forall2 {A B} (P : A -> B -> Type) : forall l1 l1' l2,
+Lemma CircularShift_R_Forall2 {A B} (P : A -> B -> Type) : forall l1 l1' l2,
   l1 ~°~ l1' -> Forall2_Type P l1 l2 -> { l2' : _ & l2 ~°~ l2' & Forall2_Type P l1' l2' }.
 Proof.
 intros l1 l1' l2 HP; revert l2.
-apply decomp_CyclicPerm_R in HP as [[lx ly] Hx Hy]; subst.
+apply decomp_CircularShift_R in HP as [[lx ly] Hx Hy]; subst.
 intros l2' HF ; inversion HF ; subst.
 - exists nil ; auto.
   + reflexivity.
@@ -349,18 +349,18 @@ intros l2' HF ; inversion HF ; subst.
   + apply Forall2_Type_app_inv_l in X0 as ([(la & lb) H1 H2] & Heq).
     simpl in Heq ; rewrite Heq.
     exists (lb ++ y :: la).
-    * rewrite app_comm_cons ; apply CyclicPerm_R_commu.
+    * rewrite app_comm_cons ; apply CircularShift_R_commu.
     * apply Forall2_Type_app ; auto.
       constructor ; auto.
 Defined.
 
 
 (* Cyclic Permutations as Nat *)
-Definition app_cperm_nat {A} n (l : list A) :=
+Definition app_cshift_nat {A} n (l : list A) :=
   skipn n l ++ firstn n l.
 
-Lemma app_cperm_cfun {A} : forall n (l : list A), n <= length l ->
-  app_cperm_nat n l = app_nat_fun (cfun n (length l - n)) l.
+Lemma app_cshift_cfun {A} : forall n (l : list A), n <= length l ->
+  app_cshift_nat n l = app_nat_fun (cfun n (length l - n)) l.
 Proof.
   intros n l Hle.
   rewrite<- (firstn_skipn n l) at 3.
@@ -371,8 +371,8 @@ Proof.
   rewrite firstn_length_le; try assumption; lia.
 Qed.
 
-Lemma cond_cyclicPerm_to_app_cperm : forall p, cond_cyclicPerm p ->
-  { n & forall {A} (l : list A), length p = length l -> app_nat_fun p l = app_cperm_nat n l}.
+Lemma cond_circularShift_to_app_cshift : forall p, cond_circularShift p ->
+  { n & forall {A} (l : list A), length p = length l -> app_nat_fun p l = app_cshift_nat n l}.
 Proof with try reflexivity.
   intros p Hperm.
   destruct Hperm as [[[n m] Heq]| Heq].
@@ -381,21 +381,21 @@ Proof with try reflexivity.
     rewrite Heq in Hlen |- *.
     rewrite cfun_length in Hlen.
     replace (S m) with (length l - S n) by lia.
-    rewrite app_cperm_cfun...
+    rewrite app_cshift_cfun...
     lia.
   - split with (length p).
     intros A l Hlen.
     rewrite Heq at 1; rewrite Hlen.
     rewrite app_Id.
-    unfold app_cperm_nat.
+    unfold app_cshift_nat.
     rewrite skipn_all2 by lia.
     rewrite firstn_all2 by lia...
 Qed.
 
-Lemma app_cperm_to_cond_cyclicPerm : forall n len,
-  {p : _ & cond_cyclicPerm p
+Lemma app_cshift_to_cond_circularShift : forall n len,
+  {p : _ & cond_circularShift p
          & prod (length p = len)
-                (forall {A} (l : list A), length p = length l -> app_nat_fun p l = app_cperm_nat n l)}.
+                (forall {A} (l : list A), length p = length l -> app_nat_fun p l = app_cshift_nat n l)}.
 Proof with try reflexivity.
   intros n len.
   destruct n; [ | case_eq ((S n) <? len); intros H ; [apply Nat.ltb_lt in H | apply Nat.ltb_nlt in H] ].
@@ -406,7 +406,7 @@ Proof with try reflexivity.
       rewrite seq_length in Hlen.
       rewrite Hlen.
       rewrite app_Id.
-      unfold app_cperm_nat; simpl.
+      unfold app_cshift_nat; simpl.
       rewrite app_nil_r...
   - split with (cfun (S n) (S (pred (pred len) - n))); [ | split ].
     + left; split with (n , pred (pred len) - n)...
@@ -415,7 +415,7 @@ Proof with try reflexivity.
     + intros A l Hlen.
       rewrite cfun_length in Hlen.
       replace (S (Init.Nat.pred (Init.Nat.pred len) - n)) with (len - S n) by lia.
-      unfold app_cperm_nat.
+      unfold app_cshift_nat.
       rewrite <- (firstn_skipn (S n) l) at 1.
       rewrite<- (firstn_length_le l) at 1 by lia.
       replace (len - S n) with (length (skipn (S n) l)); [apply app_cfun_eq | ].
@@ -426,7 +426,7 @@ Proof with try reflexivity.
     + intros A l Hlen.
       rewrite seq_length in Hlen; rewrite Hlen.
       rewrite app_Id.
-      unfold app_cperm_nat.
+      unfold app_cshift_nat.
       rewrite skipn_all2 by lia.
       rewrite firstn_all2 by lia...
 Qed.
